



PHY-685
QFT-1

Lecture - 31

We have obtained the E.O.M. of a Weyl Fermion in 4-component notation.

We introduce a 4-component Majorana field:

$$\Psi_M = \begin{pmatrix} \psi_c \\ \psi^\dagger c \end{pmatrix} \quad \text{The upper and lower component are the same Weyl field.}$$

The previous E.O.M. becomes $(i \gamma^\mu \partial_\mu - m \mathbb{1}_{4 \times 4}) \Psi_M = 0$

This is Dirac's eqn for Majorana field.

Now let's consider two left handed Weyl field with an $SO(2)$ symmetry:

$$\mathcal{L} = i \psi_i^\dagger \bar{\sigma}^\mu \partial_\mu \psi_i - \frac{1}{2} m \psi_i \psi_i - \frac{1}{2} \psi_i^\dagger \psi_i^\dagger$$

This Lagrangian is invariant under an $SO(2)$ transformation

$$\begin{pmatrix} \psi'_1 \\ \psi'_2 \end{pmatrix} = \begin{pmatrix} \cos \alpha & \sin \alpha \\ -\sin \alpha & \cos \alpha \end{pmatrix} \begin{pmatrix} \psi_1 \\ \psi_2 \end{pmatrix}.$$

The $SO(2)$ invariance appears as $U(1)$ invariance when we write:

$$\chi = \frac{1}{\sqrt{2}} (\psi_1 + i \psi_2), \quad \xi = \frac{1}{\sqrt{2}} (\psi_1 - i \psi_2).$$

Plugging back to the original Lagrangian:

$$\mathcal{L} = i \chi^\dagger \bar{\sigma}^\mu \partial_\mu \chi + i \xi^\dagger \bar{\sigma}^\mu \partial_\mu \xi - m \chi \xi - m \xi^\dagger \chi^\dagger.$$

This \mathcal{L} is invariant under a global $U(1)$:

$$\chi \rightarrow e^{-i\alpha} \chi, \quad \xi \rightarrow e^{i\alpha} \xi.$$

Now we have the E.O.M of $\chi := \frac{\partial \mathcal{L}}{\partial \chi^\dagger} = 0$
 $\mathcal{L} \quad \quad \quad \xi = \frac{\partial \mathcal{L}}{\partial \xi^\dagger} = 0$

Following the same algebraic steps, these two simultaneous eqs can be clubbed into:

$$\begin{pmatrix} -m \delta_a^c & i \sigma_a^\mu{}_{\dot{c}} \partial_\mu \\ i \bar{\sigma}^{\mu \dot{a} c} & -m \delta_a^c \end{pmatrix} \begin{pmatrix} \chi_c \\ \xi^{\dot{a} c} \end{pmatrix} = 0$$

Now define a 4-component Dirac field $\Psi_D = \begin{pmatrix} \chi_a \\ \xi^{\dot{a} c} \end{pmatrix}$

This also has the E.O.M as Dirac's eqs.

$$\Psi_D^\dagger = (\chi_a^\dagger, \xi^a) := \text{Hermitian conjugation.}$$

Then introduce: $\beta = \begin{pmatrix} 0 & \delta_a^{\dot{c}} \\ \delta_a^c & 0 \end{pmatrix}$. using this

$$\begin{aligned} \text{we define } \bar{\Psi}_D &= \Psi_D^\dagger \beta = (\chi_a^\dagger, \xi^a) \begin{pmatrix} 0 & \delta_a^{\dot{c}} \\ \delta_a^c & 0 \end{pmatrix} \\ &= (\xi^c, \chi^{\dot{c}}) \end{aligned}$$

β and γ^0 are numerically same (modulo an i), but has different spinor structure.

$$\text{So } \bar{\Psi}_D \Psi_D = (\xi^c, \chi^{\dot{c}}) \begin{pmatrix} \chi_c \\ \xi^{\dot{c}} \end{pmatrix} = \xi^c \chi_c + \chi^{\dot{c}} \xi^{\dot{c}}$$

using these forms:

$$\bar{\Psi}_D \gamma^\mu \partial_\mu \Psi_D = \xi^a \sigma_a^\mu{}_{\dot{c}} \partial_\mu \xi^{\dot{c}} + \chi^{\dot{a}} \bar{\sigma}^{\mu \dot{a} c} \partial_\mu \chi_c$$

$$\text{Now } \xi^a \sigma_a^\mu{}_{\dot{c}} \partial_\mu \xi^{\dot{c}} = \partial_\mu [\xi^a \sigma_a^\mu{}_{\dot{c}} \xi^{\dot{c}}] - (\partial_\mu \xi^a) \sigma_a^\mu{}_{\dot{c}} \xi^{\dot{c}}$$

So the first term can be written as

$$\begin{aligned}
 -(\partial_\mu \xi^a) \sigma_{ac}^\mu \xi^\dagger{}^c &= -(\partial_\mu \varepsilon^{ab} \psi_b) \sigma_{ac}^\mu \psi_b^\dagger \varepsilon^{bc} \\
 &= +\psi_b^\dagger \varepsilon^{bc} \varepsilon^{ab} \sigma_{ac}^\mu (\partial_\mu \psi_b) \\
 &= +\psi_b^\dagger \varepsilon^{bc} \varepsilon_{c,d} \bar{\sigma}^{\mu d b} (\partial_\mu \psi_b) \\
 &= \psi_b^\dagger \delta_{d,b} \bar{\sigma}^{\mu d b} (\partial_\mu \psi_b) \\
 &= \psi_b^\dagger \bar{\sigma}^{\mu d b} \partial_\mu \psi_b
 \end{aligned}$$

Hence

$$\bar{\Psi}_D \gamma^\mu \partial_\mu \Psi_D = \chi^\dagger \bar{\sigma}^\mu \partial_\mu \chi + \xi^\dagger \bar{\sigma}^\mu \partial_\mu \xi + \partial_\mu (\xi \sigma^\mu \xi^\dagger)$$

Hence upto a total divergence

$$\mathcal{L}_D = i \bar{\Psi}_D \gamma^\mu \partial_\mu \Psi_D - m \bar{\Psi}_D \Psi_D$$

This is invariant under a global UCD $\Psi_D \rightarrow e^{-i\alpha} \Psi_D$ and $\bar{\Psi}_D \rightarrow e^{i\alpha} \bar{\Psi}_D$. (H.W. compute the Noether current).

There is an additional discrete symmetry called charge conjugation, which exchanges χ and ξ .

It operates as

$$\begin{aligned}
 C^{-1} \chi_a(x) C &= \xi_a(x) \\
 C^{-1} \xi_a(x) C &= \chi_a(x)
 \end{aligned}$$

$$\left\{ \begin{aligned} C^\dagger &= C^\dagger = C^{-1} = -C \\ C &= \begin{pmatrix} -i\sigma^2 & \\ & i\sigma^2 \end{pmatrix} \end{aligned} \right.$$

One can show $C^{-1} \mathcal{L}(x) C = \mathcal{L}(x)$

$$C = \begin{pmatrix} \varepsilon_{ac} & 0 \\ 0 & \varepsilon^{ac} \end{pmatrix}$$

$$\bar{\Psi}_D^T = \begin{pmatrix} \xi^c \\ \chi^\dagger{}^c \end{pmatrix}, \quad \Psi_D^c = C \bar{\Psi}_D^T = \begin{pmatrix} \varepsilon_{ac} & 0 \\ 0 & \varepsilon^{ac} \end{pmatrix} \begin{pmatrix} \xi^c \\ \chi^\dagger{}^c \end{pmatrix} = \begin{pmatrix} \xi_a \\ \chi^\dagger{}^a \end{pmatrix}$$

Comparing side-by-side.

$$\psi_D = \begin{pmatrix} \chi_c \\ \xi + i \end{pmatrix}, \quad \psi_D^c = \begin{pmatrix} \xi_c \\ \chi + i \end{pmatrix}$$

Now $C^{-1} \psi_D(x) C \quad | \quad C^{-1} = \begin{pmatrix} \epsilon^{ba} & \\ & \epsilon_{ia} \end{pmatrix}$

This leads to $C^{-1} \gamma^\mu C = -(\gamma^\mu)^T.$

For a Majorana field $\boxed{\psi_M^c = C^{-1} \psi_M C = \psi_M}$. Its analogous

to the $\phi^\dagger = \phi$ for a real scalar field.

The original Lagrangian of the single left-handed Weyl fermion was

$$\mathcal{L} = i \psi^\dagger \bar{\sigma}^\mu \partial_\mu \psi - \frac{1}{2} m \psi \psi + \text{h.c.}$$

$$= \frac{i}{2} \psi^\dagger \bar{\sigma}^\mu \partial_\mu \psi + \frac{i}{2} \psi \sigma^\mu \partial_\mu \psi^\dagger - \frac{1}{2} m \psi \psi - \frac{1}{2} m \psi^\dagger \psi^\dagger$$

Now $\bar{\psi}_M = (\psi_M^c \psi_M^\dagger)^c$, so replacing $\chi \rightarrow \psi$ and $\xi \rightarrow \psi$ in the Dirac Lagrangian,

$$\mathcal{L}_M = \frac{i}{2} \bar{\psi}_M \gamma^\mu \partial_\mu \psi_M - \frac{1}{2} m \bar{\psi}_M \psi_M$$

For Majorana fermions, $\bar{\psi} = \psi^T C$, so

$$\mathcal{L}_M = \frac{i}{2} \psi_M^T C \gamma^\mu \partial_\mu \psi_M - \frac{1}{2} m \psi_M^T C \psi_M.$$

The projection operators are constructed using

$$\gamma_5 \equiv \begin{pmatrix} -\delta_a^c & 0 \\ 0 & +\delta_a^c \end{pmatrix}$$

$$P_L = \frac{1}{2}(1 - \gamma_5) = \begin{pmatrix} \delta_a^c & 0 \\ 0 & 0 \end{pmatrix} \text{ and } P_R = \frac{1}{2}(1 + \gamma_5) = \begin{pmatrix} 0 & 0 \\ 0 & \delta_a^c \end{pmatrix}$$

This defines $\psi_L \equiv P_L \psi = \begin{pmatrix} \chi_c \\ 0 \end{pmatrix}$ & $\psi_R \equiv P_R \psi = \begin{pmatrix} 0 \\ \xi + i \end{pmatrix}$

$$\gamma_5 = \frac{i}{4!} \epsilon_{\mu\nu\rho\sigma} \gamma^\mu \gamma^\nu \gamma^\rho \gamma^\sigma$$

Now let's remember that if $\Psi_D = \begin{pmatrix} \chi_a \\ \xi^{\dagger a} \end{pmatrix}$, then

$$\bar{\Psi}_D = (\xi^c, \chi^{\dagger c}). \text{ So when } \Psi_L = \begin{pmatrix} \chi_a \\ 0 \end{pmatrix}, \bar{\Psi}_L = (0, \chi^{\dagger a}).$$

$$\text{and } \Psi_R = \begin{pmatrix} 0 \\ \xi^{\dagger a} \end{pmatrix} \Rightarrow \bar{\Psi}_R = (\xi^a, 0)$$

$$\text{Now } \mathcal{L}_D = i \chi^{\dagger} \bar{\sigma}^{\mu} \partial_{\mu} \chi + i \xi^{\dagger} \bar{\sigma}^{\mu} \partial_{\mu} \xi - m \chi \xi - m \xi^{\dagger} \chi^{\dagger}.$$

$$\begin{aligned} \text{So the Dirac fermion has mass term } m \bar{\Psi}_D \Psi_D \\ &= m \chi \xi + m \xi^{\dagger} \chi^{\dagger} \\ &= m \xi^a \chi_a + m \chi^{\dagger a} \xi^{\dagger a} \\ &= m (\bar{\Psi}_R \Psi_L + \bar{\Psi}_L \Psi_R). \end{aligned}$$

So Ψ_L and Ψ_R only mixes through mass terms and E.O.M.
Hence massless fermions are helicity eigen-states.

$$\text{Now we have this grand equation of free fields} \\ (i \gamma^{\mu} \partial_{\mu} - m) \Psi_D = 0$$

This is a "classical E.O.M" of free fields which transforms under $(\frac{1}{2}, 0)$ and $(0, \frac{1}{2})$ representation of $SL(2, \mathbb{C})$. First obvious question how do we solve it?

It's a matrix equation $\underbrace{\hspace{1cm}}_{4 \times 4 \text{ diff operator}} (\psi) = 0 \rightarrow 4 \times 1 \text{ null matrix} \rightarrow (4 \times 1) \text{ function}$

First let's multiply from left by $(i \gamma^{\nu} \partial_{\nu} + m)$ to get:

$$\begin{aligned} &[i \gamma^{\nu} \partial_{\nu} + m][i \gamma^{\mu} \partial_{\mu} - m] \psi = 0 \\ \Rightarrow &[-\partial^{\nu} \partial_{\nu} \gamma^{\nu} \gamma^{\mu} + i m \gamma^{\mu} \partial_{\mu} - i m \gamma^{\nu} \partial_{\nu} - m^2] \psi = 0 \\ \Rightarrow &[-\partial^{\nu} \partial_{\nu} \gamma^{\nu} \gamma^{\mu} + m^2] \psi = 0 \\ \Rightarrow &[-\partial^{\nu} \partial_{\nu} \left(\frac{1}{2} \{ \gamma^{\nu}, \gamma^{\mu} \} + \frac{1}{2} [\gamma^{\nu}, \gamma^{\mu}] \right) + m^2] \psi = 0 \end{aligned}$$

$$\Rightarrow \left(\frac{1}{2} \partial^2 \partial_\mu \cdot 2 \gamma^{\mu 2} + m^2 \right) \psi = 0$$

$$\Rightarrow (\partial^2 + m^2) \psi = 0 \Rightarrow \psi \text{ satisfy K-G. eqs. as well.}$$

we know that solution of these equations are plane waves $e^{-i\vec{p} \cdot \vec{x}}$ and $e^{i\vec{p} \cdot \vec{x}}$ where $p^0 = \sqrt{\vec{p}^2 + m^2}$.

Let's write the generic solution as linear superpositions of these two plane waves:

$$\psi_s(x) = \int \frac{d^4 p}{(2\pi)^4} \delta^4(p^2 - m^2) \theta(p^0) u_s(p) e^{-i\vec{p} \cdot \vec{x}}$$

$$\text{and } \chi_s(x) = \int \frac{d^4 p}{(2\pi)^4} \delta^4(p^2 - m^2) \theta(p^0) v_s(p) e^{i\vec{p} \cdot \vec{x}}$$

When we plug these solutions in Dirac's eqs we get

$$\begin{pmatrix} -m & \vec{p} \cdot \vec{\sigma} \\ \vec{p} \cdot \vec{\sigma} & -m \end{pmatrix} u_s(p) = 0 \text{ and } \begin{pmatrix} -m & -\vec{p} \cdot \vec{\sigma} \\ -\vec{p} \cdot \vec{\sigma} & -m \end{pmatrix} v_s(p) = 0$$

Let's look at this equation in the rest frame $p^\mu = (m, \vec{0})$.
We have $\vec{p}^\mu \equiv \vec{p}^\mu$

$$m \begin{pmatrix} -1 & 1 \\ 1 & -1 \end{pmatrix} u_s(\vec{p}^\mu) = 0 \text{ and } m \begin{pmatrix} -1 & -1 \\ -1 & -1 \end{pmatrix} v_s(\vec{p}^\mu) = 0$$

$$\text{So the solutions are constants } u_s = \sqrt{m} \begin{pmatrix} \xi_s \\ \xi_s \end{pmatrix}, v_s = \sqrt{m} \begin{pmatrix} \eta_s \\ -\eta_s \end{pmatrix}$$

We conventionally normalize ξ to have $\xi^\dagger \xi = 1$, same for η .

Dirac fermion is a 4-complex number object which can be written in the basis of

$$u_+ = \sqrt{m} \begin{pmatrix} 1 \\ 0 \\ 0 \\ 1 \end{pmatrix}, u_- = \sqrt{m} \begin{pmatrix} 0 \\ 1 \\ 0 \\ 1 \end{pmatrix}, v_+ = \sqrt{m} \begin{pmatrix} -1 \\ 0 \\ 1 \\ 0 \end{pmatrix}, v_- = \sqrt{m} \begin{pmatrix} 0 \\ 1 \\ 0 \\ -1 \end{pmatrix}$$

Now in a general boosted frame $p^\mu = (E, 0, 0, p_z)$

$$\vec{p} \cdot \vec{\sigma} = \begin{pmatrix} E - p_z & 0 \\ 0 & E + p_z \end{pmatrix} \text{ and } \vec{p} \cdot \vec{\sigma} = \begin{pmatrix} E + p_z & 0 \\ 0 & E - p_z \end{pmatrix}$$

Let $a = \sqrt{E - p_z}$ and $b = \sqrt{E + p_z}$, then $a^2 b^2 = E^2 - p_z^2 = m^2$

Now the eqs
$$\begin{pmatrix} -m \mathbb{1}_{2 \times 2} & p \cdot \sigma \\ p \cdot \sigma & -m \mathbb{1}_{2 \times 2} \end{pmatrix} u_s(p) = 0, \text{ become}$$

$$\begin{pmatrix} -m & 0 & E - p_z & 0 \\ 0 & -m & 0 & E + p_z \\ E + p_z & 0 & -m & 0 \\ 0 & E - p_z & 0 & -m \end{pmatrix} u_s(p) = 0$$

$$\Rightarrow \begin{pmatrix} -ab & b & a^2 & 0 \\ 0 & -ab & 0 & b^2 \\ b^2 & 0 & -ab & 0 \\ 0 & a^2 & 0 & -ab \end{pmatrix} u_s(p) = 0$$

The solutions are:
$$u_s = \begin{pmatrix} \begin{pmatrix} a & 0 \\ \sigma & b \end{pmatrix} \xi_s \\ \begin{pmatrix} b & 0 \\ \sigma & a \end{pmatrix} \xi_s \end{pmatrix}$$

$$\Rightarrow u_s(p) = \begin{bmatrix} \begin{pmatrix} \sqrt{E - p_z} & 0 \\ 0 & \sqrt{E + p_z} \end{pmatrix} \xi_s \\ \begin{pmatrix} \sqrt{E + p_z} & 0 \\ 0 & \sqrt{E - p_z} \end{pmatrix} \xi_s \end{bmatrix} = \begin{bmatrix} \sqrt{p \cdot \sigma} \xi_s \\ \sqrt{p \cdot \bar{\sigma}} \xi_s \end{bmatrix}$$

$$v_s(p) = \begin{bmatrix} \begin{pmatrix} \sqrt{E - p_z} & 0 \\ 0 & \sqrt{E + p_z} \end{pmatrix} \eta_s \\ \begin{pmatrix} -\sqrt{E + p_z} & 0 \\ 0 & -\sqrt{E - p_z} \end{pmatrix} \eta_s \end{bmatrix} = \begin{bmatrix} \sqrt{p \cdot \sigma} \eta_s \\ -\sqrt{p \cdot \bar{\sigma}} \eta_s \end{bmatrix}$$

check $\bar{u}_s(p) u_{s'}(p) = 2m \delta_{ss'}$, $\bar{v}_s(p) v_{s'}(p) = -2m \delta_{ss'}$

$\sum_s u_s \bar{u}_s = \not{p} + m$ and $\sum_s v_s \bar{v}_s = \not{p} - m$.